src/named/Compilers.v
@@ -50,6 +50,90 @@ Section WithVar.
     Notation compile_args := (compile_args (V_Eqb:=V_Eqb) (tgt_Model:=tgt_Model)).
     Notation compile_subst := (compile_subst (V_Eqb:=V_Eqb) (tgt_Model:=tgt_Model)).
     Notation compile_ctx := (compile_ctx (V_Eqb:=V_Eqb) (tgt_Model:=tgt_Model)).
+
+
+  (* Adds some facts that can be derived from wfness of the language
+     for a full compiler (not an extension)
+     and are helpful to the proof.
+   *)
+  Inductive preserving_compiler_plus : compiler _ -> lang -> Prop :=
+  | preserving_compiler_nil : preserving_compiler_plus [] []
+  | preserving_compiler_sort : forall cmp l n c args t,
+      preserving_compiler_plus cmp l ->
+      Model.wf_ctx (compile_ctx cmp c) ->
+      (* Notable: only uses the previous parts of the compiler on c *)
+      Model.wf_sort (compile_ctx cmp c) t ->
+      preserving_compiler_plus ((n,sort_case (map fst c) t)::cmp)
+                              ((n,sort_rule c args) :: l)
+  | preserving_compiler_term : forall cmp l n c args e t,
+      preserving_compiler_plus cmp l ->
+      Model.wf_ctx (compile_ctx cmp c) ->
+      (* Notable: only uses the previous parts of the compiler on c, t *)
+      Model.wf_term (compile_ctx cmp c) e (compile_sort cmp t) ->
+      preserving_compiler_plus ((n, term_case (map fst c) e)::cmp)
+                              ((n,term_rule c args t) :: l)
+  | preserving_compiler_sort_eq : forall cmp l n c t1 t2,
+      preserving_compiler_plus cmp l ->
+      Model.wf_ctx (compile_ctx cmp c) ->
+      (* Notable: only uses the previous parts of the compiler on c *)
+      Model.eq_sort (compile_ctx cmp c)
+              (compile_sort cmp t1)
+              (compile_sort cmp t2) ->
+      preserving_compiler_plus cmp ((n,sort_eq_rule c t1 t2) :: l)
+  | preserving_compiler_term_eq : forall cmp l n c e1 e2 t,
+      preserving_compiler_plus cmp l ->
+      Model.wf_ctx (compile_ctx cmp c) ->
+      (* Notable: only uses the previous parts of the compiler on c *)
+      Model.eq_term (compile_ctx cmp c)
+              (compile_sort cmp t)
+              (compile cmp e1)
+              (compile cmp e2) ->
+      preserving_compiler_plus cmp ((n,term_eq_rule c e1 e2 t) :: l).
+
+  Lemma invert_preserving_compiler_plus_nil cmp
+    : preserving_compiler_plus cmp [] <-> cmp = [].
+  Proof. solve_invert_constr_eq_lemma. Qed.
+  Hint Rewrite invert_preserving_compiler_plus_nil : lang_core.
+
+  Lemma invert_preserving_compiler_plus_sort_rule n c args t cmp l
+    : preserving_compiler_plus ((n,sort_case (map fst c) t)::cmp)
+                               ((n,sort_rule c args) :: l)
+      <-> preserving_compiler_plus cmp l /\
+            Model.wf_ctx (compile_ctx cmp c) /\
+            Model.wf_sort (compile_ctx cmp c) t.
+  Proof. solve_invert_constr_eq_lemma. Qed.
+  Hint Rewrite invert_preserving_compiler_plus_sort_rule : lang_core.
+
+  Lemma invert_preserving_compiler_plus_term_rule n c args e t cmp l
+    : preserving_compiler_plus ((n,term_case (map fst c) e)::cmp)
+                               ((n,term_rule c args t) :: l)
+      <-> preserving_compiler_plus cmp l /\
+            Model.wf_ctx (compile_ctx cmp c) /\
+            Model.wf_term (compile_ctx cmp c) e (compile_sort cmp t).
+  Proof. solve_invert_constr_eq_lemma. Qed.
+    Hint Rewrite invert_preserving_compiler_plus_term_rule : lang_core.
+
+    
+  Lemma invert_preserving_compiler_plus_sort_eq_rule n c t1 t2 cmp l
+    : preserving_compiler_plus cmp ((n,sort_eq_rule c t1 t2) :: l)
+      <-> preserving_compiler_plus cmp l /\
+            Model.wf_ctx (compile_ctx cmp c) /\
+            Model.eq_sort (compile_ctx cmp c)
+                          (compile_sort cmp t1)
+                          (compile_sort cmp t2).
+  Proof. solve_invert_constr_eq_lemma. Qed.
+    Hint Rewrite invert_preserving_compiler_plus_sort_eq_rule : lang_core.
+    
+  Lemma invert_preserving_compiler_plus_term_eq_rule n c e1 e2 t cmp l
+    : preserving_compiler_plus cmp ((n,term_eq_rule c e1 e2 t) :: l)
+      <-> preserving_compiler_plus cmp l /\
+            Model.wf_ctx (compile_ctx cmp c) /\
+            Model.eq_term (compile_ctx cmp c)
+                          (compile_sort cmp t)
+                          (compile cmp e1)
+                          (compile cmp e2).
+  Proof. solve_invert_constr_eq_lemma. Qed.
+  Hint Rewrite invert_preserving_compiler_plus_term_eq_rule : lang_core.
   
 Lemma fresh_compile_ctx x cmp c
   : fresh x (compile_ctx cmp c) <-> fresh x c.
@@ -69,8 +153,8 @@ Qed.
 Hint Rewrite all_fresh_compile_ctx : lang_core.
 
 
-Lemma fresh_lang_fresh_cmp cmp_pre cmp l n
-  : preserving_compiler_ext cmp_pre cmp l ->
+Lemma fresh_lang_fresh_cmp cmp l n
+  : preserving_compiler_plus cmp l ->
     fresh n l -> fresh n cmp.
 Proof.
   induction 1; basic_goal_prep;
@@ -80,7 +164,7 @@ Hint Resolve fresh_lang_fresh_cmp : lang_core.
 
 
 Lemma all_fresh_compiler cmp l
-  : preserving_compiler_ext [] cmp l ->
+  : preserving_compiler_plus cmp l ->
     all_fresh l ->
     all_fresh cmp.
 Proof.
@@ -152,8 +236,8 @@ Qed.
 Hint Rewrite compile_strengthen_ctx : lang_core.
 
 
-Lemma sort_name_in_cmp cmp_pre cmp src c' args n
-  : preserving_compiler_ext cmp_pre cmp src ->
+Lemma sort_name_in_cmp cmp src c' args n
+  : preserving_compiler_plus cmp src ->
     In (n, sort_rule c' args) src ->
     In n (map fst cmp).
 Proof.
@@ -162,8 +246,8 @@ Proof.
 Qed.
 Local Hint Resolve sort_name_in_cmp : lang_core.
 
-Lemma term_name_in_cmp cmp_pre cmp src c' args t n
-  : preserving_compiler_ext cmp_pre cmp src ->
+Lemma term_name_in_cmp cmp src c' args t n
+  : preserving_compiler_plus cmp src ->
     In (n, term_rule c' args t) src ->
     In n (map fst cmp).
 Proof.
@@ -173,7 +257,7 @@ Qed.
 Local Hint Resolve term_name_in_cmp : lang_core.
                    
 Local Lemma all_constructors_from_wf cmp src
-  : preserving_compiler_ext [] cmp src ->
+  : preserving_compiler_plus cmp src ->
     (forall c t,
         wf_sort src c t ->
         all_constructors_sort (fun n0 : V => In n0 (map fst cmp)) t)
@@ -188,20 +272,20 @@ Proof.
     with_rule_in_wf_crush.
 Qed.
 
-Definition all_constructors_sort_from_wf cmp src (pr : preserving_compiler_ext [] cmp src)
+Definition all_constructors_sort_from_wf cmp src (pr : preserving_compiler_plus cmp src)
   := proj1 (all_constructors_from_wf pr).
 Hint Resolve all_constructors_sort_from_wf : lang_core.
 
-Definition all_constructors_term_from_wf cmp src (pr : preserving_compiler_ext [] cmp src)
+Definition all_constructors_term_from_wf cmp src (pr : preserving_compiler_plus cmp src)
   := proj1 (proj2 (all_constructors_from_wf pr)).
 Hint Resolve all_constructors_term_from_wf : lang_core.
 
-Definition all_constructors_args_from_wf cmp src (pr : preserving_compiler_ext [] cmp src)
+Definition all_constructors_args_from_wf cmp src (pr : preserving_compiler_plus cmp src)
   := proj2 (proj2 (all_constructors_from_wf pr)).
 Hint Resolve all_constructors_args_from_wf : lang_core.
 
 Lemma all_constructors_ctx_from_wf cmp src c
-  : preserving_compiler_ext [] cmp src ->
+  : preserving_compiler_plus cmp src ->
     wf_ctx src c ->
     all_constructors_ctx (fun n0 : V => In n0 (map fst cmp)) c.
 Proof.
@@ -210,43 +294,230 @@ Proof.
 Qed.
 Hint Resolve all_constructors_ctx_from_wf : lang_core.
 
+    (*TODO: experimental*)
 
-(*TODO: think about whether this should be generalized*)
-Lemma inductive_implies_semantic_sort_axiom ls cmp name c t1 t2
-  : preserving_compiler_ext [] cmp ls -> wf_lang ls ->
-    In (name, sort_eq_rule c t1 t2) ls ->
-    Model.eq_sort (compile_ctx cmp c) (compile_sort cmp t1) (compile_sort cmp t2).
+    (*TODO: move to defs*)
+    Definition ws_compiler_case (c : compiler_case V) :=
+      match c with
+      | sort_case c t =>
+          well_scoped (Substable:=sort_substable (Model:=tgt_Model)) c t
+      | term_case c e =>
+          well_scoped (Substable:= @substable0_is_substable _ _ (term_substable (Model:=tgt_Model))) c e
+      end.
+
+    Definition ws_compiler : compiler V -> Prop :=
+      all (fun p => ws_compiler_case (snd p)).
+    
+    Section WithModelOk.
+      Context {tgt_Model_ok : Model_ok tgt_Model}.
+
+
+      (*TODO: generalize proofs to all models
+#[export] Hint Resolve eq_subst_subst_monotonicity : lang_core.
+#[export] Hint Resolve wf_args_subst_monotonicity : lang_core.
+       *)
+      (*TODO: Add to Model.v*)
+Local Hint Resolve wf_sort_subst_monotonicity : lang_core.
+Local Hint Resolve wf_term_subst_monotonicity : lang_core.
+Local Hint Resolve wf_sort_implies_ws : lang_core.
+      Local Hint Resolve wf_term_implies_ws : lang_core.
+
+      (*TODO: move to Substable*)
+      Lemma well_scoped_change_args V' A B `{@Substable0 V' A} `{S : @Substable V' A B} (a:B) args args'
+        : well_scoped (Substable := S) args' a ->
+          args = args' ->
+          well_scoped args a.
+      Proof.  
+        intros; subst; auto.
+      Qed.
+      Hint Resolve well_scoped_change_args : term.
+      
+    Lemma preserving_compiler_ws cmp ls
+      : preserving_compiler_plus cmp ls ->
+        ws_compiler cmp.
+    Proof.
+      induction 1; basic_goal_prep; basic_core_crush.
+      {
+        eapply well_scoped_change_args.
+        typeclasses eauto.
+        eapply Model.wf_sort_implies_ws; eauto.
+        unfold compile_ctx.
+        rewrite named_map_fst_eq.
+        reflexivity.
+      }
+      {
+        eapply well_scoped_change_args.
+        typeclasses eauto.
+        eapply Model.wf_term_implies_ws; eauto.
+        unfold compile_ctx.
+        rewrite named_map_fst_eq.
+        reflexivity.
+      }
+    Qed.      
+
+      
+      Lemma preserving_compiler_tail cmp l' l
+        : preserving_compiler_plus cmp (l' ++ l) ->
+          exists cmp' cmp_pre,
+            cmp = cmp'++ cmp_pre
+            /\ (preserving_compiler_plus cmp_pre l).
+      Proof.
+        revert cmp.
+        induction l';
+          basic_goal_prep.
+        {
+          exists [], cmp;
+            basic_core_crush.
+        }
+        {
+          inversion H1; clear H1; subst;
+          specialize (IHl' _ H6); break; subst.
+          1,2: let x1 := open_constr:(_::_) in
+               exists x1; eexists; basic_utils_crush.
+          all: eexists; eexists; basic_utils_crush.
+        }
+      Qed.
+
+Lemma compile_subst_lookup cmp s n
+  : compile cmp (subst_lookup s n)
+  = Substable.subst_lookup (compile_subst cmp s) n.
 Proof.
-  induction 1;
-    basic_goal_prep; try use_rule_in_wf;
-    basic_core_firstorder_crush.    
-  (*TODO: why is this needed? should be automated*)
-  all: use_rule_in_wf;autorewrite with lang_core utils in *;
-    intuition eauto with lang_core.
-  (*TODO: fix automation to handle this*)
-  eapply all_constructors_ctx_from_wf; eassumption.
-  eapply all_constructors_ctx_from_wf; eassumption.
-Qed.
-
-
-Lemma inductive_implies_semantic_term_axiom ls cmp name c e1 e2 t
-  : preserving_compiler_ext [] cmp ls -> wf_lang ls ->
-    In (name, term_eq_rule c e1 e2 t) ls ->
-    Model.eq_term (compile_ctx cmp c) (compile_sort cmp t) (compile cmp e1) (compile cmp e2).
-Proof.
-  induction 1;
+  induction s;
     basic_goal_prep;
-    try use_rule_in_wf;
-    basic_core_firstorder_crush.
-  (*TODO: why is this needed? should be automated*)
-  all: use_rule_in_wf;autorewrite with lang_core utils in *;
-    intuition eauto with lang_core.
-  (*TODO: fix automation to handle this*)
-  eapply all_constructors_ctx_from_wf; eassumption.
-  eapply all_constructors_ctx_from_wf; eassumption.
+    basic_core_crush.
+  case_match; basic_core_crush.
 Qed.
+Hint Rewrite compile_subst_lookup : lang_core.
 
+      (*TODO: move to Utils.v*)
+      Lemma map_fst_combine_r_padded {A B} `{WithDefault B} (l1 : list A) (l2 : list B)
+        : map fst (combine_r_padded l1 l2) = l1.
+      Proof.
+        revert l2; induction l1; destruct l2;
+          basic_goal_prep; repeat case_match; basic_utils_crush.
+      Qed.
 
+      Lemma named_map_combine_r_padded {A B C} `{WithDefault B} `{WithDefault C}
+            (l1 : list A) (l2 : list B) (f : B -> C)
+        : f default = default ->
+          Utils.named_map f (combine_r_padded l1 l2) = combine_r_padded l1 (map f l2).
+      Proof.
+        intros; revert l2; induction l1; destruct l2; basic_goal_prep; basic_utils_crush.
+        f_equal; [ congruence|].
+        rewrite IHl1.
+        reflexivity.
+      Qed.
+
+      
+    Lemma combine_r_padded_eq_len {A B} `{WithDefault B} (l1 : list A) (l2 : list B)
+      : length l1 = length l2 ->
+        combine_r_padded l1 l2 = combine l1 l2.
+      Proof.
+        revert l2; induction l1; destruct l2;
+          basic_goal_prep; repeat case_match; basic_utils_crush.
+      Qed.
+      
+      (*TODO: where to put these?*)
+      Context (sort_default_subst : forall s, (default : tgt_sort)[/s/] = (default : tgt_sort)).
+      Context (term_default_subst : forall s, (default : tgt_term)[/s/] = (default : tgt_term)).
+      
+      Local Lemma distribute_compile_subst_term cmp (s : subst) e
+        : ws_compiler cmp ->
+          all_fresh cmp ->
+          well_scoped (map fst s) e ->
+          compile cmp e[/s/] = (compile cmp e)[/compile_subst cmp s/].
+      Proof.
+        induction e.
+        {
+          simpl.
+          (*TODO: wrap subst_var for better rewriting*)
+          unfold apply_subst.
+          simpl.
+          erewrite Substable.subst_var; try typeclasses eauto.
+          intros; apply compile_subst_lookup.
+        }
+        {
+          simpl.
+          intros.
+          case_match; auto.
+          case_match; auto.
+          erewrite subst_assoc; try typeclasses eauto.
+          2:{                                              
+            rewrite map_fst_combine_r_padded.
+            apply named_list_lookup_err_in in HeqH5.
+            exact (in_all _ _ H2 HeqH5).
+          }
+          f_equal.
+          unfold subst_cmp.
+          rewrite named_map_combine_r_padded.
+          {
+            f_equal.
+            rewrite !map_map.
+            revert H4 H3 H2 H1.
+            induction l;
+              basic_goal_prep; auto;
+              autorewrite with utils in *;
+              intuition idtac.
+          }
+          {
+            apply term_default_subst.
+          }
+        }
+      Qed.
+      Hint Rewrite distribute_compile_subst_term : lang_core.
+
+      Local Lemma distribute_compile_subst_args cmp (s : subst) e
+        : ws_compiler cmp ->
+          all_fresh cmp ->
+          well_scoped (map fst s) e ->
+          compile_args cmp e[/s/] = (compile_args cmp e)[/compile_subst cmp s/].
+      Proof.
+        induction e; auto; basic_goal_prep;
+          intuition eauto.
+        f_equal; eauto.
+        apply distribute_compile_subst_term; eauto.
+      Qed.
+      Hint Rewrite distribute_compile_subst_args : lang_core.
+
+      Local Lemma distribute_compile_subst_sort cmp (s : subst) t
+        : ws_compiler cmp ->
+          all_fresh cmp ->
+          well_scoped (map fst s) t ->
+          compile_sort cmp t[/s/] = (compile_sort cmp t)[/compile_subst cmp s/].
+      Proof.
+        destruct t.
+        {
+          simpl.
+          intros.
+          case_match; auto.
+          case_match; auto.
+          erewrite subst_assoc; try typeclasses eauto.
+          2:{                                              
+            rewrite map_fst_combine_r_padded.
+            apply named_list_lookup_err_in in HeqH4.
+            exact (in_all _ _ H1 HeqH4).
+          }
+          f_equal.
+          unfold subst_cmp.
+          rewrite named_map_combine_r_padded.
+          {
+            f_equal.
+            rewrite !map_map.
+            revert H3 H2 H1.
+            induction l;
+              basic_goal_prep; auto;
+              autorewrite with utils in *;
+              intuition idtac.
+            apply distribute_compile_subst_term; eauto.
+          }
+          {
+            apply term_default_subst.
+          }
+        }
+      Qed.
+      Hint Rewrite distribute_compile_subst_sort : lang_core.
+
+      
 Lemma with_names_from_compile_ctx (A:Type) cmp c (s : list A)
   : with_names_from (compile_ctx cmp c) s
     = with_names_from c s.
@@ -256,754 +527,644 @@ Proof.
   cbn.
   f_equal; basic_core_crush.
 Qed.
-  
 
-
-
-Lemma compile_id_args A cmp (c : named_list A)
-  : map (compile cmp) (id_args c) = id_args c.
+      (* TODO: duplicated in Core. Move both to Model*)
+Lemma wf_subst_from_wf_args c s c'
+  : Model.wf_args c s c' ->
+    Model.wf_subst c (with_names_from c' s) c'.
 Proof.
-  unfold id_args.
-  induction c; 
-    basic_goal_prep;
-    basic_core_crush.
+  induction 1; basic_core_crush.
 Qed.
-Hint Rewrite compile_id_args : lang_core.
+      Hint Resolve wf_subst_from_wf_args : lang_core.
 
-Lemma fst_equal_id_args_equal A B (c1 : named_list A) (c2 : named_list B)
-  : map fst c1 = map fst c2 -> id_args c1 = id_args c2.
-Proof.
-  unfold id_args; basic_core_crush.
-Qed.
-
-Lemma compile_ctx_fst_equal cmp c
-  : map fst (compile_ctx cmp c) = map fst c.
-Proof.
-  induction c; break; simpl; f_equal; auto.
-Qed.
- 
-
-Lemma inductive_implies_semantic_sort_rule_id ls cmp name c args
-  : preserving_compiler_ext [] cmp ls -> wf_lang ls ->
-    In (name, sort_rule c args) ls ->
-    Model.wf_sort (compile_ctx cmp c) (compile_sort cmp (scon name (id_args c))).
-Proof.
-  induction 1;
-      basic_goal_prep;
-      with_rule_in_wf_crush.
-  all: try eapply all_constructors_ctx_from_wf; eauto with lang_core.
-  {
-    my_case Hname (eqb name n);[|case_match]; basic_core_firstorder_crush.
-  }
-  {
-    use_rule_in_wf; basic_core_crush.
-  }
-  {
-    my_case Hname (eqb name n);[|case_match]; basic_core_crush.
-  }
-  4:{
-    use_rule_in_wf; basic_core_crush.
-  }
-  (*TODO: eqb? where did this come from?*)
-  all: constructor.
-Qed.
-
-
-
-Lemma inductive_implies_semantic_term_rule_id ls cmp name c args t
-  : preserving_compiler_ext [] cmp ls -> wf_lang ls ->
-    In (name, term_rule c args t) ls ->
-    Model.wf_term (compile_ctx cmp c) (compile cmp (con name (id_args c))) (compile_sort cmp t).
-Proof.
-  induction 1;
-      basic_goal_prep;
-      try use_rule_in_wf;
-      basic_core_firstorder_crush.
-  all: try solve [use_rule_in_wf; basic_core_crush].
-  {
-    my_case Hname (eqb name n);[|case_match]; basic_core_crush.
-  }
-  {
-    (*TODO: fix automation to handle this*)
-    use_rule_in_wf; basic_core_crush.
-    eapply all_constructors_ctx_from_wf; eassumption.
-  }
-  {
-    (*TODO: fix automation to handle this*)
-    eapply all_constructors_ctx_from_wf; eassumption.
-  }
-  {
-    my_case Hname (eqb name n);[|case_match]; basic_core_crush.
-  }
-  {
-    (*TODO: fix automation to handle this*)
-    use_rule_in_wf; basic_core_crush.
-    eapply all_constructors_ctx_from_wf; eassumption.
-  }
-Qed.
-
-
-
-Lemma lookup_in_dom s n
-  : In n (map fst s) -> In (subst_lookup s n) (map snd s).
-Proof.
-  induction s;
-    basic_goal_prep;
-    basic_core_crush.
-  case_match; basic_core_crush.
-Qed.
-
-(*
-Lemma wf_con_id_args_subst' A (c : named_list A) s
-  : forall n e, In n (map fst c) ->
-                In n (map fst s) ->
-                In e (id_args c)[/s/] -> In e (map snd s).
-Proof.
-  induction c;
-    basic_goal_prep;
-    basic_core_crush.
-  (apply lookup_in_dom; assumption).
-  
-  
-  rewrite IHc.
-  unfold args_subst.
-*)
-
-(*TODO: move subst_lookup to Substable.v
-  so that RHS here can call subst_lookup
- *)
-Lemma compile_subst_lookup cmp s n
-  : compile cmp (subst_lookup s n)
-  = named_list_lookup (inj_var n) (compile_subst cmp s) n.
-Proof.
-  induction s;
-    basic_goal_prep;
-    basic_core_crush.
-  case_match; basic_core_crush.
-Qed.
-Hint Rewrite compile_subst_lookup : lang_core.
-
-
-Lemma combine_subst args l s
-  : (combine args l)[/s/] = combine args l[/s/].
-Proof.
-  revert args.
-  induction l;
-    destruct args;
-    basic_goal_prep;
-    basic_core_crush.
-Qed.
-
-
-Lemma lang_compiler_sort_case_args_eq cmp_pre cmp ls n c args args' e
-  : preserving_compiler_ext cmp_pre cmp ls ->
-    all_fresh ls ->
-    In (n, sort_rule c args) ls ->
-    In (n, sort_case args' e) cmp ->
-    args' = map fst c.
-Proof.
-  induction 1; basic_goal_prep; basic_core_crush.
-  match goal with
-    [Hp : preserving_compiler_ext _ _ _,
-          H : fresh _ _|-_]=>
-    pose proof (fresh_lang_fresh_cmp Hp H)
-  end.
-  basic_core_crush.
-Qed.
-Hint Resolve lang_compiler_sort_case_args_eq : lang_core.
-
-Lemma lang_compiler_term_case_args_eq cmp_pre cmp ls n c args args' e t
-  : preserving_compiler_ext cmp_pre cmp ls ->
-    all_fresh ls ->
-    In (n, term_rule c args t) ls ->
-    In (n, term_case args' e) cmp ->
-    args' = map fst c.
-Proof.
-  (*TODO: takes a long time*)
-  induction 1; basic_goal_prep; basic_core_firstorder_crush.
-  match goal with
-    [Hp : preserving_compiler_ext _ _ _,
-          H : fresh _ _|-_]=>
-    pose proof (fresh_lang_fresh_cmp Hp H)
-  end.
-  basic_core_crush.
-Qed.
-Hint Resolve lang_compiler_term_case_args_eq : lang_core.    
-
-Lemma sort_case_in_preserving_well_scoped cmp_pre cmp src n args t
-  : preserving_compiler_ext cmp_pre cmp src ->
-    (*ws_lang tgt ->*)
-    In (n, sort_case args t) cmp ->
-    well_scoped args t.
-Proof.
-  induction 1; basic_goal_prep; basic_core_firstorder_crush.
-  erewrite <- compile_ctx_fst_equal.
-  eapply wf_sort_implies_ws; eauto; eauto with term lang_core.
-Qed.
-Hint Resolve sort_case_in_preserving_well_scoped : lang_core.
-
-
-Lemma term_case_in_preserving_well_scoped cmp_pre cmp src n args t
-  : preserving_compiler_ext cmp_pre cmp src ->
-    (*ws_lang tgt ->*)
-    In (n, term_case args t) cmp ->
-    well_scoped args t.
-Proof.
-  induction 1; basic_goal_prep; basic_core_firstorder_crush.
-  erewrite <- compile_ctx_fst_equal.
-  eapply wf_term_implies_ws; eauto; eauto with term lang_core.
-Qed.
-Hint Resolve term_case_in_preserving_well_scoped : lang_core.
-
-(*TODO: move to term?
-  TODO: make type inference smoother
-
-  TODO: do I need this for Model default? I'd prefer not
- *)
-    Lemma subst_term_default s
-      : (@default term (@term_default V _) : term)[/s/]
-        = (@default term (@term_default V _) : term).
-    Proof.
-      unfold default.
-      unfold term_default.
-      simpl.
-      reflexivity.
-    Qed.
-    Hint Rewrite subst_term_default : lang_core.
-    
-    (*TODO: move to term?
-  TODO: make type inference smoother
-
-  TODO: do I need this for Model default? I'd prefer not
-     *)
-    Lemma subst_sort_default s
-      : (@default sort (@sort_default V _) : sort)[/s/]
-        = (@default sort (@sort_default V _) : sort).
-    Proof.
-      unfold default.
-      unfold sort_default.
-      simpl.
-      reflexivity.
-    Qed.
-    Hint Rewrite subst_sort_default : lang_core.
-    (* TODO: move to Substable.v (and remove dup from Term.v*)
-   
-Local Lemma distribute_compile_subst cmp src (s : subst)
-  : preserving_compiler_ext [] cmp src ->
-    all_fresh src ->
-    (forall (c : ctx) t,
-        wf_sort src c t ->
-        map fst c = map fst s ->
-        compile_sort cmp t[/s/] = (compile_sort cmp t)[/compile_subst cmp s/])
-    /\ (forall (c : ctx) e t,
-           wf_term src c e t ->
-           map fst c = map fst s ->
-           compile cmp e[/s/] = (compile cmp e)[/compile_subst cmp s/])
-    /\ (forall (c : ctx) (s' : list term) (c' : ctx),
-           wf_args src c s' c' ->
-           map fst c = map fst s ->
-           compile_args cmp s'[/s/] = (compile_args cmp s')[/compile_subst cmp s/]).
-Proof.
-  intros; apply wf_judge_ind; 
-    basic_goal_prep;
-    basic_core_crush.
-  {
-    case_match; basic_core_crush.
-    case_match; basic_core_firstorder_crush.
-    1,4:admit (*TODO: what to do about defaults?*).
-    all:lazymatch goal with
-        [ H1 : preserving_compiler_ext [] ?cmp ?src,
-            H2 : all_fresh ?src,
-              H3 : In _ ?src,
-              H4 : In _ ?cmp |- _] =>
-          pose proof (lang_compiler_sort_case_args_eq _ _ _ _ _ H1 H2 H3 H4)
-      end;
-      basic_core_firstorder_crush.
-    {
-      match goal with
-        [H : compile_args _ _ = _|-_] =>
-        unfold compile_args in H;
-          rewrite H
-      end.
-      erewrite Substable.with_names_from_args_subst.
-      reflexivity.
-    }
-  }
-  {
-    case_match; basic_core_crush.
-    case_match; basic_core_firstorder_crush.
-    3,4:admit (*TODO: what to do about defaults?*).
-    all:lazymatch goal with
-        [ H1 : preserving_compiler_ext [] ?cmp ?src,
-            H2 : all_fresh ?src,
-              H3 : In _ ?src,
-              H4 : In _ ?cmp |- _] =>
-          pose proof (lang_compiler_term_case_args_eq _ _ _ _ _ _ H1 H2 H3 H4)
-      end; basic_core_firstorder_crush.
-    {
-      fold_Substable.
-      match goal with
-        [H : compile_args _ _ = _|-_] =>
-        unfold compile_args in H;
-          rewrite H
-      end.
-      erewrite Substable.with_names_from_args_subst.
-      reflexivity.
-    }
-  }
-  admit (*TODO: add axiom to Substable about subst and inj_var *).
-  (*Qed.*)
-Admitted.
-
-Lemma compile_term_subst cmp src s c e t
-  : preserving_compiler_ext [] cmp src ->
-    all_fresh src ->
-    wf_term src c e t ->
-    map fst c = map fst s ->
-    compile cmp e[/s/] = (compile cmp e)[/compile_subst cmp s/].
-Proof.
-  intros; eapply distribute_compile_subst; eassumption.
-Qed.
-Hint Rewrite compile_term_subst : lang_core.
-
-
-Lemma compile_sort_subst cmp src s c t
-  : preserving_compiler_ext [] cmp src ->
-    all_fresh src ->
-    wf_sort src c t ->
-    map fst c = map fst s ->
-    compile_sort cmp t[/s/] = (compile_sort cmp t)[/compile_subst cmp s/].
-Proof.
-  intros; eapply distribute_compile_subst; eassumption.
-Qed.
-Hint Rewrite compile_sort_subst : lang_core.
-
-
-Lemma compile_args_subst cmp src s c s' c'
-  : preserving_compiler_ext [] cmp src ->
-    all_fresh src ->
-    wf_args src c s' c' ->
-    map fst c = map fst s ->
-    compile_args cmp s'[/s/] = (compile_args cmp s')[/compile_subst cmp s/].
-Proof.
-  intros; eapply distribute_compile_subst; eassumption.
-Qed.
-Hint Rewrite compile_args_subst : lang_core.
-
-Lemma compile_subst_with_names_from A cmp (c':named_list A) s
-  : (compile_subst cmp (with_names_from c' s)) = with_names_from c' (map (compile cmp) s).
-Proof.
-  unfold compile_subst.
-  rewrite <- with_names_from_map_is_named_map.
-  reflexivity.
-Qed.
-
-Lemma compile_scon cmp args s name t
-  : all_fresh cmp ->
-    In (name, sort_case args t) cmp ->
-    (compile_sort cmp (scon name s)) = t[/(combine args (compile_args cmp s))/].
-Proof.
-  basic_goal_prep; repeat case_match; basic_core_crush.
-  {
-    (*TODO: should be automated; how best to do so?*)
-    lazymatch goal with
-      [ H : all_fresh ?cmp, H0 : In _ ?cmp, H1 : In _ ?cmp |-_]=>
-        pose proof (in_all_fresh_same _ _ _ _ H H0 H1)
-    end.
-    basic_core_crush.
-  }
-  {
-    (*TODO: should be automated; how best to do so?*)
-    lazymatch goal with
-      [ H : all_fresh ?cmp, H0 : In _ ?cmp, H1 : In _ ?cmp |-_]=>
-        pose proof (in_all_fresh_same _ _ _ _ H H0 H1)
-    end.
-    basic_core_crush.
-  }
-  {
-    exfalso.
-    (*TODO: why isn't this automated already?*)
-    eapply named_list_lookup_none; eauto.
-  }
-Qed.
-  
-Lemma lang_compiler_conflict_sort_term cmp_pre cmp ls n c args args' e
-  : preserving_compiler_ext cmp_pre cmp ls ->
-    all_fresh ls ->
-    In (n, sort_rule c args) ls ->
-    In (n, term_case args' e) cmp ->
-    False.
-Proof.
-  induction 1; basic_goal_prep; basic_core_crush.
-  match goal with
-    [Hp : preserving_compiler_ext _ _ _,
-          H : fresh _ _|-_]=>
-    pose proof (fresh_lang_fresh_cmp Hp H)
-  end.
-  basic_core_crush.
-Qed.
-Hint Resolve lang_compiler_conflict_sort_term : lang_core.
-
-  
-Lemma lang_compiler_conflict_term_sort cmp_pre cmp ls n c args args' e t
-  : preserving_compiler_ext cmp_pre cmp ls ->
-    all_fresh ls ->
-    In (n, term_rule c args t) ls ->
-    In (n, sort_case args' e) cmp ->
-    False.
-Proof.
-  induction 1; basic_goal_prep; basic_core_firstorder_crush.
-  match goal with
-    [Hp : preserving_compiler_ext _ _ _,
-          H : fresh _ _|-_]=>
-    pose proof (fresh_lang_fresh_cmp Hp H)
-  end.
-  eauto with utils.
-Qed.
-Hint Resolve lang_compiler_conflict_term_sort : lang_core.
-  
-
-Lemma inductive_implies_semantic_sort_rule ls cmp name c c' args s
-  : preserving_compiler_ext [] cmp ls -> wf_lang ls ->
-    In (name, sort_rule c' args) ls ->
-    Model.wf_ctx (compile_ctx cmp c') ->
-    Model.wf_args (compile_ctx cmp c) (compile_args cmp s) (compile_ctx cmp c') ->
-    Model.wf_sort (compile_ctx cmp c) (compile_sort cmp (scon name s)).
-Proof.
-  intros.
-  replace (scon name s) with (scon name (id_args c'))[/(with_names_from c' s)/].
-  erewrite compile_sort_subst; try eassumption; eauto with lang_core.
-  2:{
-    econstructor; [eassumption |].
-    basic_core_crush.
-  }
-  (*TODO: need this axiom for models *)
-  eapply wf_sort_subst_monotonicity; auto.
-  {
-    eapply inductive_implies_semantic_sort_rule_id; eauto.
-  }
-  all: basic_core_firstorder_crush.
-  {
-    rewrite compile_subst_with_names_from.
-    erewrite <- with_names_from_compile_ctx.
-    eapply wf_subst_from_wf_args; basic_core_crush.
-  }
-  {
-    pose proof (wf_args_length_eq H4).
-    unfold compile_args in H5.
-    unfold compile_ctx in H5.
-    basic_core_crush.
-  }
-  {
-    simpl; f_equal.
-    rewrite wf_con_id_args_subst; basic_core_firstorder_crush.
-    rewrite <- all_fresh_compile_ctx.
-    eauto with lang_core.
-    pose proof (wf_args_length_eq H4).
-    unfold compile_args in H5.
-    unfold compile_ctx in H5.
-    basic_core_crush.
-  }
-Qed.
-
-Lemma inductive_implies_semantic_term_rule ls lt cmp name c c' args t s
-  : wf_lang lt -> preserving_compiler_ext [] lt cmp ls -> wf_lang ls ->
-    In (name, term_rule c' args t) ls ->
-    wf_ctx lt (compile_ctx cmp c') ->
-    wf_args lt (compile_ctx cmp c) (compile_args cmp s) (compile_ctx cmp c') ->
-    wf_term lt (compile_ctx cmp c) (compile cmp (con name s)) (compile_sort cmp t)[/compile_subst cmp (with_names_from c' s)/].
-Proof.
-  intros.
-  replace (con name s) with (con name (id_args c'))[/(with_names_from c' s)/].
-  erewrite compile_term_subst; try eassumption; eauto with lang_core.
-  2:{
-    econstructor; [eassumption |].
-    basic_core_crush.
-  }
-  eapply wf_term_subst_monotonicity; auto.
-  {
-    eapply inductive_implies_semantic_term_rule_id; eauto.
-  }
-  {
-    basic_core_crush.
-  }
-  {
-    rewrite compile_subst_with_names_from.
-    erewrite <- with_names_from_compile_ctx.
-    eapply wf_subst_from_wf_args; basic_core_crush.
-  }
-  {
-    pose proof (wf_args_length_eq H4).
-    unfold compile_args in H5.
-    unfold compile_ctx in H5.
-    basic_core_firstorder_crush.
-  }
-  {
-    simpl; f_equal.
-    fold_Substable.
-    rewrite wf_con_id_args_subst; basic_core_firstorder_crush.
-    rewrite <- all_fresh_compile_ctx.
-    eauto with lang_core.
-    pose proof (wf_args_length_eq H4).
-    unfold compile_args in H5.
-    unfold compile_ctx in H5.
-    basic_core_crush.
-  }
-Qed.
-
-
+(*      
 (*TODO: maybe not necessary with better strengthening lemma?
   See what happens when I use the better one
 *)
-Variant rule_compiles_with {lt cmp} : rule -> Prop :=
+Variant rule_compiles_with {cmp} : rule -> Prop :=
 | sort_rule_compiles_with c args
-  : wf_ctx lt (compile_ctx cmp c) -> rule_compiles_with (sort_rule c args)
+  : Model.wf_ctx (compile_ctx cmp c) -> rule_compiles_with (sort_rule c args)
 | term_rule_compiles_with c args t
-  : wf_ctx lt (compile_ctx cmp c) ->
-    wf_sort lt (compile_ctx cmp c) (compile_sort cmp t) ->
+  : Model.wf_ctx (compile_ctx cmp c) ->
+    Model.wf_sort (compile_ctx cmp c) (compile_sort cmp t) ->
     rule_compiles_with (term_rule c args t)
 (*Similar properties are not necessary for eq rules*)
 | sort_eq_rule_compiles_with c t1 t2 : rule_compiles_with (sort_eq_rule c t1 t2)
 | term_eq_rule_compiles_with c e1 e2 t : rule_compiles_with (term_eq_rule c e1 e2 t).
 Arguments rule_compiles_with : clear implicits.
                        
-Definition lang_compiles_with lt cmp : lang -> Prop :=
-  all (fun p => rule_compiles_with lt cmp (snd p)).
+Definition lang_compiles_with cmp : lang -> Prop :=
+  all (fun p => rule_compiles_with cmp (snd p)).
+*)
 
+      Lemma wf_lang_tail l' l
+        : wf_lang (l' ++ l) -> wf_lang l.
+      Proof.
+        induction l';
+          basic_goal_prep;
+          basic_core_crush.
+      Qed.
 
-Lemma lang_compiles_with_sort_ctx_in lt cmp ls n c' args
-  : lang_compiles_with lt cmp ls ->
-    In (n, sort_rule c' args) ls ->
-    wf_ctx lt (compile_ctx cmp c').
-Proof.
-  induction ls; 
-    basic_goal_prep;
-    basic_core_firstorder_crush.
-  (*TODO: This could be automated w/ an inversion lemma*)
-  match goal with
-    [H : rule_compiles_with _ _ _ |-_]=>
-    inversion H; basic_core_crush
-  end.
-Qed.
-Local Hint Resolve lang_compiles_with_sort_ctx_in : lang_core.
+      Lemma all_fresh_tail {A} (l1 l2: named_list A)
+        : all_fresh (l1++l2) -> all_fresh l2.
+      Proof.
+        induction l1; basic_goal_prep; basic_utils_crush.
+      Qed.
 
-Lemma lang_compiles_with_term_ctx_in lt cmp ls n c' args t
-  : lang_compiles_with lt cmp ls ->
-    In (n, term_rule c' args t) ls ->
-    wf_ctx lt (compile_ctx cmp c').
-Proof.
-  induction ls; 
-    basic_goal_prep;
-    basic_core_firstorder_crush.
-  (*TODO: This could be automated w/ an inversion lemma*)
-  match goal with
-    [H : rule_compiles_with _ _ _ |-_]=>
-    inversion H; basic_core_crush
-  end.
-Qed.
-Local Hint Resolve lang_compiles_with_term_ctx_in : lang_core.
+      Lemma all_fresh_conflict_impossible {A} (l1 l2: named_list A) n a1 a2
+        : all_fresh (l1++l2) -> In (n,a1) l1 -> In (n,a2) l2 -> False.
+      Proof.
+        induction l1; basic_goal_prep; basic_utils_crush.
+      Qed.
+      Hint Resolve all_fresh_conflict_impossible : utils.
 
-Lemma lang_compiles_with_term_sort_in lt cmp ls n c' args t
-  : lang_compiles_with lt cmp ls ->
-    In (n, term_rule c' args t) ls ->
-    wf_sort lt (compile_ctx cmp c') (compile_sort cmp t).
-Proof.
-  induction ls; 
-    basic_goal_prep;
-    basic_core_firstorder_crush.
-  (*TODO: This could be automated w/ an inversion lemma*)
-  match goal with
-    [H : rule_compiles_with _ _ _ |-_]=>
-    inversion H; basic_core_crush
-  end.
-Qed.
-Local Hint Resolve lang_compiles_with_term_sort_in : lang_core.
+       Lemma in_twice_appended_all_fresh {A} (l1 l2: named_list A) n a
+              : all_fresh (l1++l2) ->
+                In (n,a) l1 ->
+                ~In n (map fst l2).
+      Proof.
+        induction l1;
+          basic_goal_prep;
+          basic_utils_crush.
+      Qed.
 
+      (*TODO: this is better than the one in utils*)
+      Lemma named_list_lookup_none {A} (l : named_list A) s
+        : None = named_list_lookup_err l s <-> fresh s l.
+      Proof.
+        induction l; basic_goal_prep; basic_utils_crush.
+        cbv; intuition.
+        my_case Hs (eqb s v); basic_goal_prep; basic_utils_crush.
+        my_case Hs (eqb s v); basic_goal_prep; basic_utils_crush.
+      Qed.
+      
+      Lemma strengthening cmp' cmp l
+        : preserving_compiler_plus cmp l ->
+          all_fresh (cmp'++cmp) ->
+          (forall c t, wf_sort l c t ->
+                        compile_sort (cmp'++cmp) t = compile_sort cmp t)
+          /\ (forall c e t, wf_term l c e t ->
+                        compile (cmp'++cmp) e = compile cmp e)
+          /\ (forall c s c', wf_args l c s c' ->
+                        compile_args (cmp'++cmp) s = compile_args cmp s).
+      Proof.
+        intros; apply wf_judge_ind;
+          basic_goal_prep;
+          basic_core_crush.
+        all: pose proof (all_fresh_tail _ _ ltac:(eassumption)).
+        all: repeat case_match; auto;
+            autorewrite with utils term lang_core in *; eauto.
+        all: basic_utils_crush.
+        all: try (pose proof (in_all_fresh_same _ _ _ _ H6 HeqH1 H7) as H';
+                  now inversion H').
+        {
+          pose proof (in_all_fresh_same _ _ _ _ H6 HeqH1 H7) as H';
+            inversion H'; clear H'; subst.
+          unfold compile_args in H5; rewrite H5.
+          reflexivity.
+        }
+        {
+          exfalso.
+          eapply named_list_lookup_none in HeqH1.
+          intuition eauto;
+            pose proof (sort_name_in_cmp _ _ _ H1 H3).
+          eapply in_twice_appended_all_fresh; eauto.
+        }
+        {
+          exfalso.
+          eapply named_list_lookup_none in HeqH1.
+          pose proof (sort_name_in_cmp _ _ _ H1 H3).
+          basic_utils_crush.
+        }
+        {
+          exfalso.
+          eapply named_list_lookup_none in HeqH7.
+          intuition eauto;
+            pose proof (sort_name_in_cmp _ _ _ H1 H3).
+          basic_utils_crush.
+        }
+        {
+          pose proof (in_all_fresh_same _ _ _ _ H6 HeqH1 H7) as H';
+            inversion H'; clear H'; subst.
+          unfold compile_args in H5; rewrite H5.
+          reflexivity.
+        }
+        {
+          exfalso.
+          eapply named_list_lookup_none in HeqH1.
+          intuition eauto;
+            pose proof (term_name_in_cmp _ _ _ _ H1 H3).
+          eapply in_twice_appended_all_fresh; eauto.
+        }
+        {
+          exfalso.
+          eapply named_list_lookup_none in HeqH1.
+          pose proof (term_name_in_cmp _ _ _ _ H1 H3).
+          basic_utils_crush.
+        }
+        {
+          exfalso.
+          eapply named_list_lookup_none in HeqH7.
+          pose proof (term_name_in_cmp _ _ _ _ H1 H3).
+          basic_utils_crush.
+        }
+      Qed.
 
-Local Lemma inductive_implies_semantic' lt cmp ls
-  : wf_lang ls ->
-    wf_lang lt ->
-    preserving_compiler_ext [] lt cmp ls ->
-    lang_compiles_with lt cmp ls ->
-    semantics_preserving lt cmp ls.
-Proof.
-  intros; apply judge_ind; 
-    basic_goal_prep;
-    basic_core_firstorder_crush.
+      Lemma strengthening_term cmp' cmp l
+        : preserving_compiler_plus cmp l ->
+          all_fresh (cmp'++cmp) ->
+          forall c e t, wf_term l c e t ->
+                        compile (cmp'++cmp) e = compile cmp e.
+      Proof.
+        intros; eapply strengthening; eauto.
+      Qed.
+      
+      Lemma strengthening_sort cmp' cmp l
+        : preserving_compiler_plus cmp l ->
+          all_fresh (cmp'++cmp) ->
+          forall c t, wf_sort l c t ->
+                        compile_sort (cmp'++cmp) t = compile_sort cmp t.
+      Proof.
+        intros; eapply strengthening; eauto.
+      Qed.
+      
+      Lemma strengthening_args cmp' cmp l
+        : preserving_compiler_plus cmp l ->
+          all_fresh (cmp'++cmp) ->
+          forall c s c', wf_args l c s c' ->
+                        compile_args (cmp'++cmp) s = compile_args cmp s.
+      Proof.
+        intros; eapply strengthening; eauto.
+      Qed.
+      
+      Lemma strengthening_ctx cmp' cmp l
+        : preserving_compiler_plus cmp l ->
+          all_fresh (cmp'++cmp) ->
+          forall c, wf_ctx l c ->
+                        compile_ctx (cmp'++cmp) c = compile_ctx cmp c.
+      Proof.
+        induction 3;
+          basic_goal_prep; f_equal; eauto; f_equal;
+          eapply strengthening_sort; eauto.
+      Qed.
+
+          (*TODO: move up*)
+      Hint Resolve preserving_compiler_ws : lang_core.
+      
+    Lemma preserving_contradiction cmp l n r c
+      : preserving_compiler_plus cmp l ->
+        all_fresh l ->        
+        In (n,r) l ->
+        In (n,c) cmp ->
+        match r,c with
+        | term_rule _ _ _, term_case _ _
+        | sort_rule _ _, sort_case _ _ => True
+        | _,_ => False
+        end.
+    Proof.
+      induction 1;
+        basic_goal_prep;
+        repeat case_match;
+        subst;
+        autorewrite with utils in *;
+        try tauto;
+        intuition (subst;try congruence; eauto with lang_core).
+      all: assert (fresh n cmp) by eauto with lang_core;
+        basic_utils_crush.
+    Qed.
+
+      Lemma sort_case_in_preserving cmp ls name
+        : preserving_compiler_plus cmp ls ->
+          wf_lang ls ->
+          forall c args t args0,
+          In (name, sort_rule c args) ls ->
+          In (name, sort_case args0 t) cmp ->
+          (args0 = (map fst c)
+           /\ Model.wf_ctx (compile_ctx cmp c)
+           /\ Model.wf_sort (compile_ctx cmp c) t).
+      Proof.
+        induction 1;
+          basic_goal_prep;
+          autorewrite with utils term lang_core in *;
+          try assumption;
+          try tauto.
+        {
+          destruct H5; destruct H6; break; subst.
+          now eauto.
+          {
+            exfalso.
+            eapply fresh_lang_fresh_cmp in H4; eauto.
+            exfalso; eauto using pair_fst_in.
+          }
+          exfalso; now eauto using pair_fst_in.
+          now eauto.
+        }
+        basic_core_crush.
+        basic_core_crush.
+        {
+          eapply all_constructors_ctx_from_wf; eauto.
+          intuition subst;
+            autorewrite with utils lang_core term in *;
+            break;
+            subst.
+          all: try assumption.
+          {
+            use_rule_in_wf.
+            basic_core_crush.
+          }
+          {
+            use_rule_in_wf.
+            basic_core_crush.
+          }
+        }
+        {
+            destruct H5; destruct H6; break; subst.
+            now eauto.
+            {
+              exfalso.
+              eapply fresh_lang_fresh_cmp in H4; eauto.
+            }
+            exfalso; now eauto using pair_fst_in.
+            now eauto.
+        }
+        now basic_core_crush. 
+        now basic_core_crush.
+        {
+          eapply all_constructors_ctx_from_wf; eauto.
+          intuition subst;
+            autorewrite with utils lang_core term in *;
+            break;
+            subst.
+          all: try assumption.
+          all: try tauto.
+          {
+            use_rule_in_wf.
+            basic_core_crush.
+          }
+        }
+        {
+          destruct H5; try tauto; break; eauto.
+        }
+        {
+          destruct H5; try tauto; break; eauto.
+        }
+      Qed.
+
+      Lemma term_case_in_preserving cmp ls name
+        : preserving_compiler_plus cmp ls ->
+          wf_lang ls ->
+          forall c args args0 e t,
+          In (name, term_rule c args t) ls ->
+          In (name, term_case args0 e) cmp ->
+          (args0 = (map fst c)
+           /\ Model.wf_ctx (compile_ctx cmp c)
+           /\ Model.wf_term (compile_ctx cmp c) e (compile_sort cmp t)).
+      Proof.
+        induction 1;
+          basic_goal_prep;
+          autorewrite with utils term lang_core in *;
+          try assumption;
+          try tauto.
+        {
+          destruct H5; destruct H6; break; subst.
+          now eauto.
+          {
+            exfalso.
+            eapply fresh_lang_fresh_cmp in H4; eauto.
+          }
+          exfalso; now eauto using pair_fst_in.
+          now eauto.
+        }
+        basic_core_crush.
+        basic_core_crush.
+         {
+          eapply all_constructors_sort_from_wf; eauto.
+          intuition subst;
+            autorewrite with utils lang_core term in *;
+            break;
+            subst.
+          all: try assumption.
+          all: try tauto.
+          use_rule_in_wf.
+          basic_core_crush.
+        }
+        now basic_core_crush.
+        now basic_core_crush.
+        {
+          eapply all_constructors_ctx_from_wf; eauto.
+          intuition subst;
+            autorewrite with utils lang_core term in *;
+            break;
+            subst.
+          all: try assumption.
+          all: try tauto.
+          {
+            use_rule_in_wf.
+            basic_core_crush.
+          }
+        }
+        {
+            destruct H5; destruct H6; break; subst.
+            now eauto.
+            {
+              exfalso.
+              eapply fresh_lang_fresh_cmp in H4; eauto.
+              now eauto using pair_fst_in.
+            }
+            exfalso; now eauto using pair_fst_in.
+            now eauto.
+        }
+        now basic_core_crush. 
+        now basic_core_crush.
+        
+         {
+          eapply all_constructors_sort_from_wf; eauto.
+          intuition subst;
+            autorewrite with utils lang_core term in *;
+            break;
+            subst.
+          all: try assumption.
+          all: try tauto.
+          all: eauto.
+          all:use_rule_in_wf;
+            basic_core_crush.
+        }
+        now basic_core_crush. 
+        now basic_core_crush.
+        {
+          eapply all_constructors_ctx_from_wf; eauto.
+          intuition subst;
+            autorewrite with utils lang_core term in *;
+            break;
+            subst.
+          all: try assumption.
+          all: try tauto.
+          all: use_rule_in_wf;
+            basic_core_crush.
+        }
+        {
+          destruct H5; try tauto; break; eauto.
+        }
+        {
+          destruct H5; try tauto; break; eauto.
+        }
+      Qed.
+
+      Lemma inductive_implies_semantic' cmp ls
+        : wf_lang ls ->
+          preserving_compiler_plus cmp ls ->
+          semantics_preserving cmp ls.
+      Proof.
+        intros.
+        apply judge_ind;
+          basic_goal_prep.
+        {
+          assert (all_fresh cmp) by basic_core_crush.
+          lazymatch goal with
+            [ Hin : In _ ?ls,
+                Hpres : preserving_compiler_plus _ ?ls,
+                  Hlang : wf_lang ?ls |- _] =>
+              apply in_split in Hin; break; subst;
+              apply wf_lang_tail in Hlang; break; subst;
+              apply preserving_compiler_tail in Hpres; break; subst
+          end.
+          autorewrite with utils lang_core in *.
+          break.
+          erewrite !strengthening_ctx, !strengthening_sort; eauto.
+        }
+        {
+          autorewrite with utils lang_core in *.
+          eapply Model.eq_sort_subst; eauto.
+          all: basic_core_crush.
+        }
+        {
+          eapply Model.eq_sort_refl; eauto.
+        }
+        {
+          eapply Model.eq_sort_trans; eauto.
+        }
+        {
+          eapply Model.eq_sort_sym; eauto.
+        }
+        {
+          autorewrite with utils lang_core in *.
+          eapply Model.eq_term_subst; eauto.
+          all: basic_core_crush.
+        }
+        {
+          assert (all_fresh cmp) by basic_core_crush.
+          lazymatch goal with
+            [ Hin : In _ ?ls,
+                Hpres : preserving_compiler_plus _ ?ls,
+                  Hlang : wf_lang ?ls |- _] =>
+              apply in_split in Hin; break; subst;
+              apply wf_lang_tail in Hlang; break; subst;
+              apply preserving_compiler_tail in Hpres; break; subst
+          end.
+          autorewrite with utils lang_core in *.
+          break.
+          erewrite !strengthening_ctx, !strengthening_sort, !strengthening_term; eauto.
+        }
+        {
+          eapply Model.eq_term_refl; eauto.
+        }
+        {
+          eapply Model.eq_term_trans; eauto.
+        }
+        {
+          eapply Model.eq_term_sym; eauto.
+        }
+        {
+          eapply Model.eq_term_conv; eauto.
+        }
+        {
+          constructor.
+        }
+        {
+          autorewrite with lang_core in *; intuition eauto with lang_core term.
+        }
+        {
+          repeat case_match.
+          {
+            apply named_list_lookup_err_in in HeqH7.
+            pose proof (preserving_contradiction _ _ _ ltac:(eassumption) ltac:(eauto with lang_core) H3 HeqH7)
+              as H'; inversion H'.
+          }
+          {
+            assert (all_fresh cmp) by basic_core_crush.
+            assert (wf_ctx ls c') by (use_rule_in_wf; basic_core_crush).
+            autorewrite with utils in *.
+            2: basic_core_crush.
+            pose proof (sort_case_in_preserving
+                          n  
+                          ltac:(eassumption)
+                                 ltac:(eassumption)
+                                        _ _ _ _                       
+                                        ltac:(eassumption)
+                                               ltac:(eassumption)).
+            break; subst.
+            eapply Model.wf_sort_subst_monotonicity; cycle 2.
+            {
+              rewrite combine_r_padded_eq_len.
+              rewrite combine_map_fst_is_with_names_from.
+              erewrite <- with_names_from_compile_ctx.
+              eapply wf_subst_from_wf_args.
+              eauto.
+              basic_core_crush.
+            }
+            {
+              eapply sort_case_in_preserving; eauto.
+            }
+            assumption.
+          }
+          {
+            rewrite named_list_lookup_none in HeqH7.
+
+            (*TODO: lost indentation
+            TODO: need another conclusion of lemma
+              admit (*TODO: same admit as above*).
+            } *)
+            lazymatch goal with
+              [ Hin : In _ ?ls,
+                  Hpres : preserving_compiler_plus _ ?ls,
+                    Hlang : wf_lang ?ls |- _] =>
+                apply in_split in Hin; break; subst;
+                apply wf_lang_tail in Hlang; break; subst;
+                apply preserving_compiler_tail in Hpres; break; subst
+            end.
+            inversion H3; subst.
+            exfalso; apply HeqH7.
+            basic_utils_crush.
+          }
+        }
+        {
+          case_match.
+          case_match.
+          {
+            autorewrite with utils in *; [| basic_core_crush..].
+            pose proof (term_case_in_preserving
+                          n  
+                          ltac:(eassumption)
+                                 ltac:(eassumption)
+                                        _ _ _ _ _                     
+                                        ltac:(eassumption)
+                                               ltac:(eassumption)).
+            break.
+            rewrite distribute_compile_subst_sort;
+              [| eauto with lang_core..].
+            rewrite combine_r_padded_eq_len.
+            subst.
+            rewrite combine_map_fst_is_with_names_from.
+            unfold compile_subst.
+            rewrite with_names_from_map_is_named_map.
+            eapply Model.wf_term_subst_monotonicity; eauto.
+            rewrite <- with_names_from_map_is_named_map.
+            erewrite <- with_names_from_compile_ctx.
+            eapply wf_subst_from_wf_args; eauto.
+            eapply H5; eauto.
+            {
+              use_rule_in_wf; basic_core_crush.
+            }
+            {
+              subst; basic_core_crush.
+            }
+            {
+              rewrite map_fst_with_names_from.
+              2:basic_core_crush.
+              use_rule_in_wf; basic_core_crush.              
+                                                        }
+          }
+          {
+            autorewrite with utils in *.
+            pose proof (preserving_contradiction _ _ _
+                                                 ltac:(eassumption)
+                                                        ltac:(eauto with lang_core)
+                                                               ltac:(eassumption)
+                                                                      ltac:(eassumption)) as H';
+              destruct H'.
+            basic_core_crush.            
+          }
+          {
+            rewrite named_list_lookup_none in HeqH7.
+
+            (*TODO: lost indentation
+            TODO: need another conclusion of lemma
+              admit (*TODO: same admit as above*).
+            } *)
+            lazymatch goal with
+              [ Hin : In _ ?ls,
+                  Hpres : preserving_compiler_plus _ ?ls,
+                    Hlang : wf_lang ?ls |- _] =>
+                apply in_split in Hin; break; subst;
+                apply wf_lang_tail in Hlang; break; subst;
+                apply preserving_compiler_tail in Hpres; break; subst
+            end.
+            inversion H3; subst.
+            exfalso; apply HeqH7.
+            basic_utils_crush.
+          }
+        }
   {
-    eapply inductive_implies_semantic_sort_axiom; eassumption.
+    eapply Model.wf_term_conv; eauto.
   }
   {
-    erewrite !compile_sort_subst.
-    all: try match goal with
-               [|- map fst _ = map fst _] =>
-               symmetry; eauto with lang_core
-             end.
-    all: basic_core_firstorder_crush.
-  }
-  {
-    erewrite !compile_sort_subst.
-    erewrite !compile_term_subst.
-    all: try match goal with
-               [|- map fst _ = map fst _] =>
-               symmetry; eauto with lang_core
-             end.
-    all: basic_core_firstorder_crush.
-  }
-  {
-    eapply inductive_implies_semantic_term_axiom; eassumption.
-  }
-  {
-    constructor; basic_core_firstorder_crush.
-    match goal with
-      [ H : eq_term _ _ (compile_sort _ _) _ _|-_] =>
-      erewrite !compile_sort_subst in H
-    end.
-    all: try match goal with
-               [|- map fst _ = map fst _] =>
-               symmetry; eauto with lang_core
-             end.
-    all: basic_core_firstorder_crush.
-  }
-  {
-    eapply inductive_implies_semantic_sort_rule; try eassumption.
-    all: try use_rule_in_wf; basic_core_firstorder_crush.
-  }
-  {
-    erewrite compile_sort_subst; eauto.
-    all: try match goal with
-               [|- map fst _ = map fst _] =>
-               symmetry; eauto with lang_core
-             end.
-    all: basic_core_firstorder_crush.
-    assert (wf_ctx ls c') by (use_rule_in_wf; basic_core_crush).
-    eapply inductive_implies_semantic_term_rule; try (auto;eassumption).
-    all: try use_rule_in_wf; basic_core_firstorder_crush.
+    eapply Model.wf_term_var; eauto.
+    unfold compile_ctx.
+    basic_utils_crush.
   }
   {
     constructor.
-    apply in_named_map; assumption.
   }
   {
-    constructor; basic_core_firstorder_crush.
-    match goal with
-      [ H : wf_term _ _ _ (compile_sort _ _) |-_] =>
-      erewrite !compile_sort_subst in H
-    end.
-    all: try match goal with
-               [|- map fst _ = map fst _] =>
-               symmetry; eauto with lang_core
-             end.
-    all: basic_core_firstorder_crush.
-    match goal with
-      [H : context [compile_subst _ (with_names_from _ _)]|-_] =>
-      rewrite compile_subst_with_names_from in H
-    end.
+    autorewrite with lang_core in *;
+    [| intuition eauto with lang_core term utils..].
+    constructor; intuition eauto with lang_core term utils.
+    unfold compile_subst in *.
+    unfold compile_args.
+    rewrite with_names_from_map_is_named_map.
     rewrite with_names_from_compile_ctx.
     assumption.
+    rewrite map_fst_with_names_from;
+      eauto with utils lang_core.
+  }
+  {
+    constructor.
+  }
+  {
+    autorewrite with lang_core in *;
+    [| intuition eauto with lang_core term utils..].
+    intuition eauto with lang_core term utils.
   }
 Qed.
 
-Local Lemma inductive_implies_semantic_ctx' lt cmp ls
-  : wf_lang ls ->
-    wf_lang lt ->
-    preserving_compiler_ext [] lt cmp ls ->
-    lang_compiles_with lt cmp ls ->
-    forall c : ctx, wf_ctx ls c -> wf_ctx lt (compile_ctx cmp c).
-Proof.
-  intros wfs wft pc lcw.
-  apply inductive_implies_semantic'; eauto.
-Qed.
-Local Hint Resolve inductive_implies_semantic_ctx' : lang_core.
+      
+      Lemma strengthen_preserving_compiler cmp ls
+        : wf_lang ls ->
+          preserving_compiler_ext [] cmp ls ->
+          preserving_compiler_plus cmp ls.
+      Proof.
+        intros wfl pc; revert wfl; induction pc;
+          basic_goal_prep; constructor;
+          autorewrite with utils lang_core in *.
+        all: break.
+        all: eauto with lang_core utils.
+        all: eapply inductive_implies_semantic';
+          eauto.
+      Qed.
 
+      Theorem inductive_implies_semantic cmp ls
+        : wf_lang ls ->
+          preserving_compiler_ext [] cmp ls ->
+          semantics_preserving cmp ls.
+      Proof.
+        intros.
+        apply inductive_implies_semantic'; auto.
+        apply strengthen_preserving_compiler; auto.
+      Qed.        
 
-Local Hint Constructors rule_compiles_with : lang_core.
-
-
-Local Lemma rule_compiles_extend_fresh lt cmp r n cc
-  : rule_compiles_with lt cmp r ->
-    all_constructors_rule (fun n0 : V => In n0 (map fst cmp)) r ->
-    fresh n cmp ->
-    all_fresh cmp ->
-    rule_compiles_with lt ((n,cc)::cmp) r.
-Proof.
-  inversion 1; basic_goal_prep; with_rule_in_wf_crush.
-  all: constructor.
-  all: try erewrite compile_strengthen_ctx; eauto.
-  all: try rewrite compile_strengthen_sort; eauto.
-Qed. 
-  
-Local Lemma lang_compiles_extend_fresh lt cmp ls n cc
-  : lang_compiles_with lt cmp ls ->
-    all (fun '(_,r) => all_constructors_rule (fun n0 : V => In n0 (map fst cmp)) r) ls ->
-    fresh n cmp ->
-    all_fresh cmp ->
-    lang_compiles_with lt ((n,cc)::cmp) ls.
-Proof.
-  unfold lang_compiles_with.
-  induction ls; basic_goal_prep; with_rule_in_wf_crush.
-  eapply rule_compiles_extend_fresh; eauto.
-Qed.  
-
-(*TODO: move to core with like lemmas above*)
-Lemma all_constructors_rule_from_wf tgt cmp src r
-  : preserving_compiler_ext [] tgt cmp src ->
-    wf_rule src r ->
-    all_constructors_rule (fun n0 : V => In n0 (map fst cmp)) r.
-Proof.
-  inversion 2; basic_goal_prep;
-    with_rule_in_wf_crush.
-  (*TODO: automation; need to restrict simplify?*)
-  all: eapply all_constructors_ctx_from_wf; eauto.
-Qed.
-Hint Resolve all_constructors_rule_from_wf : lang_core.
-
-
-Lemma wf_lang_implies_all_constructors lt l
-  : wf_lang l ->
-    forall cmp,
-    preserving_compiler_ext [] lt cmp l ->
-    all (fun '(_,r) => all_constructors_rule (fun n0 : V => In n0 (map fst cmp)) r) l.
-Proof.
-  induction 1; basic_goal_prep;
-    with_rule_in_wf_crush.
-  (*TODO: break down cmp*)
-  inversion H2; subst.
-  1,2:specialize (IHwf_lang_ext cmp0).
-  3,4:specialize (IHwf_lang_ext cmp).
-  all:eapply all_constructors_lang_weaken.
-  all: try apply IHwf_lang_ext; auto.
-  all:basic_goal_prep; basic_core_firstorder_crush.
-Qed.
-
-
-Local Lemma preserving_compiler_to_lang_compiles_with lt ls
-  : wf_lang ls ->
-    wf_lang lt ->
-    forall cmp,
-    preserving_compiler_ext [] lt cmp ls ->
-    lang_compiles_with lt cmp ls.
-Proof.
-  induction 1; inversion 2; basic_goal_prep; with_rule_in_wf_crush.
-  all: try constructor.
-  all: try rewrite compile_strengthen_ctx; eauto.
-  all: try rewrite compile_strengthen_sort; eauto.
-  all: try apply lang_compiles_extend_fresh; eauto with lang_core.
-  all: try eapply wf_lang_implies_all_constructors; eauto.
-  all: eapply all_constructors_ctx_from_wf; [| eauto..]; eauto.
-Qed.
-
-
-Theorem inductive_implies_semantic lt cmp ls
-  : wf_lang ls ->
-    wf_lang lt ->
-    preserving_compiler_ext [] lt cmp ls ->
-    semantics_preserving lt cmp ls.
-Proof.
-  intros; apply inductive_implies_semantic';
-    eauto using  preserving_compiler_to_lang_compiles_with.
-Qed.
-
+    End WithModelOk.
+    End WithModel.
+      
 End WithVar.
 
 
@@ -1022,20 +1183,5 @@ End WithVar.
 #[export] Hint Resolve all_constructors_term_from_wf : lang_core.
 #[export] Hint Resolve all_constructors_args_from_wf : lang_core.
 #[export] Hint Resolve all_constructors_ctx_from_wf : lang_core.
-#[export] Hint Rewrite compile_id_args : lang_core.
 #[export] Hint Rewrite compile_subst_lookup : lang_core.
 
-#[export] Hint Resolve lang_compiler_sort_case_args_eq : lang_core.
-#[export] Hint Resolve lang_compiler_term_case_args_eq : lang_core.
-#[export] Hint Resolve sort_case_in_preserving_well_scoped : lang_core.
-#[export] Hint Resolve term_case_in_preserving_well_scoped : lang_core.
-
-#[export] Hint Rewrite compile_term_subst : lang_core.
-#[export] Hint Rewrite compile_sort_subst : lang_core.
-#[export] Hint Rewrite compile_args_subst : lang_core.
-
-#[export] Hint Resolve lang_compiler_conflict_sort_term : lang_core.
-#[export] Hint Resolve lang_compiler_conflict_term_sort : lang_core.
-
-
-#[export] Hint Resolve all_constructors_rule_from_wf : lang_core.
